F_mu_ref_par/soundness_unary.v
@@ -2,41 +2,29 @@ From iris_logrel.F_mu_ref_par Require Export fundamental_unary.
 From iris.proofmode Require Import tactics pviewshifts.
 From iris.program_logic Require Import ownership adequacy.
 
-Section Soundness.
-  Let Σ := #[ auth.authGF heapUR ].
+Section soundness.
+  Definition Σ := #[ auth.authGF heapUR ].
 
-  Definition free_type_context: varC -n> valC -n> iPropG lang Σ := λne x y,
-    True%I.
-
-  Lemma wp_soundness e τ :
+  Lemma wp_soundness e τ σ :
     [] ⊢ₜ e : τ →
-    ownP ∅ ⊢ WP e {{v, ∃ H : heapIG Σ,
-      interp (nroot .@ "Fμ,ref,par" .@ 1) τ free_type_context v }}.
+    ownP σ ⊢ WP e {{ v, ∃ H : heapIG Σ, interp (nroot .@ 1) τ [] v}}.
   Proof.
     iIntros {H1} "Hemp".
-    iPvs (heap_alloc (nroot .@ "Fμ,ref,par" .@ 2) with "Hemp")
+    iPvs (heap_alloc (nroot .@ 2) with "Hemp")
       as {H} "[Hheap Hemp]"; first solve_ndisj.
     iApply wp_wand_l. iSplitR.
     { iIntros {v} "HΦ". iExists H. iExact "HΦ". }
     rewrite -(empty_env_subst e).
-    iApply (@typed_interp _ H (nroot .@ "Fμ,ref,par" .@ 1)
-                              (nroot .@ "Fμ,ref,par" .@ 2) _ _ []); eauto.
+    iApply (@typed_interp _ _ (nroot .@ 1) (nroot .@ 2)); eauto.
     solve_ndisj.
   Qed.
 
-  Theorem Soundness e τ :
-    [] ⊢ₜ e : τ →
-    ∀ e' thp h, rtc step ([e], of_heap ∅) (e' :: thp, h) →
-              ¬reducible e' h → is_Some (to_val e').
+  Theorem soundness e τ e' thp σ σ' :
+    [] ⊢ₜ e : τ → rtc step ([e], σ) (e' :: thp, σ') →
+    is_Some (to_val e') ∨ reducible e' σ'.
   Proof.
-    intros H1 e' thp h Hstp Hnr.
-    eapply wp_soundness in H1; eauto.
-    edestruct (@wp_adequacy_reducible lang (globalF Σ) ⊤ (λ v, ∃ H,
-        @interp Σ H (nroot .@ "Fμ,ref,par" .@ 1) τ free_type_context v)%I
-      e e' (e' :: thp) ∅ ∅ h) as [Ha|Ha]; eauto; try tauto.
-    - done.
-    - iIntros "[Hp Hg]". by iApply H1.
-    - by rewrite of_empty_heap in Hstp.
+    intros ??. eapply wp_adequacy_reducible; eauto using ucmra_unit_valid.
+    - iIntros "[??]". by iApply wp_soundness.
     - constructor.
   Qed.
-End Soundness.
+End soundness.
